decl let f(x) = e; fib4
git-svn-id: https://www.lri.fr/svn/demons/why2/trunk@218 ecafba89-7d34-45a1-8a0b-92829e960b72

bench/good/loops.ml
@@ -16,7 +16,7 @@ let loop1 =
 
 parameter x: int ref
 
-let oppose = fun (u:unit) -> (x := - !x) { x = -x@ }
+let oppose (u:unit) = (x := - !x) { x = -x@ }
 
 let loop2 = 
   { x <= 10 }
